Working on stack_call proof

compiler/backend/proofs/stack_callProofScript.sml
@@ -1,10 +1,16 @@
 (*
-  Kommentar som beskriver filen
+  Kommentar som beskriver filen ddd
 *)
 
-open preamble stackLangTheory stackSemTheory stack_callTheory;
+open preamble stackLangTheory stackSemTheory stack_callTheory wordLangTheory;
 
 val _ = new_theory("stack_callProof");
+
+Theorem dest_Call_NONE_INL_SOME[simp]:
+  dest_Call_NONE_INL x = SOME m <=> x = (Call NONE (INL m) NONE)
+Proof
+  cheat
+QED;
 
 Theorem dest_StackFree_SOME[simp]:
   dest_StackFree x = SOME m <=> x = StackFree m
@@ -20,13 +26,32 @@ Proof
   \\ fs[dest_StackFree_def]
 QED;
 
+val code_rel_def = Define `
+  code_rel s_code t_code tree <=>
+    !n x. lookup n s_code = SOME x ==>
+          ?m. lookup n tree = SOME m /\
+          lookup n t_code = SOME (strip_fun x (n + 1)) /\
+          lookup (n + 1) t_code = SOME (opt_code (create_raw_ep x) tree)
+`;
+
 val state_rel_def = Define `
   state_rel s t <=>
     t.clock = s.clock /\
     t.regs = s.regs /\
     t.stack = s.stack /\
     t.stack_space = s.stack_space /\
-    ARB (* TODO: complete this *)`;
+    t.use_alloc = s.use_alloc /\
+    t.bitmaps = s.bitmaps /\
+    t.fp_regs = s.fp_regs /\
+    t.store = s.store /\
+    t.memory = s.memory /\
+    t.mdomain = s.mdomain /\
+    t.gc_fun = s.gc_fun /\
+    t.use_stack = s.use_stack /\
+    t.use_store = s.use_store /\
+    t.ffi = s.ffi /\
+    t.ffi_save_regs = s.ffi_save_regs /\
+    t.be = s.be`;
 
 val tree_accurate_def = Define `
   tree_accurate tree (s_code:('a stackLang$prog) num_map) <=>
@@ -41,35 +66,100 @@ val tree_accurate_def = Define `
   <| regs := dfgdg ; clock := 3 |>
 *)
 
+Theorem word_loc_case_eq:
+  word_loc_CASE x f1 f2 = y <=>
+  (?w. x = Word w /\ f1 w = y) \/
+  ?l1 l2. x = Loc l1 l2 /\ f2 l1 l2 = y
+Proof
+  Cases_on `x` \\ fs[]
+QED;
+
+val opt_code_Seq = SIMP_CONV(srw_ss())[Once opt_code_def]``opt_code (Seq p1 p2) tree``
+
 Theorem opt_code_correct:
   !prog s res s1 t tree.
-    evaluate (prog,s) = (res,s1) /\ state_rel s t /\
+    evaluate (prog,s) = (res,s1) /\ state_rel s t /\ code_rel s.code t.code tree /\
     tree_accurate tree s.code /\ res <> SOME Error ==>
-    ?ck t1. evaluate (opt_code prog tree,t with clock := t.clock + ck) =
-              (res,t1) /\ state_rel s1 t1 /\ tree_accurate tree s1.code
+    ?ck t1. evaluate (opt_code prog tree,t with clock := t.clock + ck) = (res,t1) /\
+            state_rel s1 t1 /\ tree_accurate tree s1.code /\
+            code_rel s1.code t1.code tree
 Proof
-
   recInduct evaluate_ind \\ rpt strip_tac
   THEN1
    (rename [`Skip`]
-    \\ fs [opt_code_def,evaluate_def] \\ rveq
+    \\ fs [opt_code_def, evaluate_def] \\ rveq
     \\ qexists_tac `0` \\ fs [state_rel_def])
   THEN1
    (rename [`Halt`]
-    \\ fs [opt_code_def,evaluate_def] \\ rveq
-    \\ fs [get_var_def,state_rel_def]
-    \\ TOP_CASE_TAC \\ fs []
+    \\ fs [opt_code_def, evaluate_def]
+    \\ rveq \\ fs [get_var_def, state_rel_def]
+    \\ TOP_CASE_TAC \\ fs[]
     \\ rveq \\ fs [empty_env_def])
-  THEN1 cheat
-  THEN1 cheat
-  THEN1 cheat
-  THEN1 cheat
-  THEN1 cheat
   THEN1
-
+   (rename[`Alloc`]
+    \\ fs[opt_code_def, evaluate_def, tree_accurate_def, state_rel_def, get_var_def, alloc_def, gc_def, set_store_def, has_space_def]
+    \\ fs[bool_case_eq]
+    \\ last_x_assum (assume_tac o SYM)
+    \\ fs[option_case_eq]
+    \\ fs[bool_case_eq, option_case_eq, word_loc_case_eq, pair_case_eq]
+    \\ rveq \\ fs[empty_env_def])
+  THEN1
+   (rename [`Inst i`]
+    \\ fs[evaluate_def, opt_code_def, option_case_eq, inst_def, state_rel_def]
+    \\ Cases_on `i` \\ fs[]
+       THEN1 (rveq \\ fs[])
+       THEN1 (fs[assign_def, option_case_eq, word_exp_def]
+         \\ rveq \\ fs[set_var_def])
+       THEN1 (fs[option_case_eq]
+         \\ Cases_on `a` \\ fs[option_case_eq, bool_case_eq]
+         \\ rveq \\ fs[set_var_def, assign_def, word_exp_def, option_case_eq]
+         \\ rveq \\ fs[]
+           THEN1 (EVERY_CASE_TAC
+             \\ fs[IS_SOME_EXISTS, word_exp_def, option_case_eq]
+             \\ EVERY_CASE_TAC \\ fs[word_op_def]
+             \\ EVERY_CASE_TAC \\ rveq \\ fs[])
+           THEN1 (fs[IS_SOME_EXISTS, option_case_eq]
+             \\ Cases_on `v1` \\ fs[word_exp_def]
+             \\ EVERY_CASE_TAC \\ fs[word_exp_def, option_case_eq]
+             \\ rveq \\ fs[]
+             \\ EVERY_CASE_TAC \\ fs[word_op_def]
+             \\ EVERY_CASE_TAC \\ rveq \\ fs[])
+           \\ (EVERY_CASE_TAC
+             \\ fs[get_vars_def, get_var_def, option_case_eq]
+             \\ rveq \\ fs[]))
+       THEN1 (Cases_on `a`
+         \\ fs[option_case_eq]
+         \\ Cases_on `m`
+         \\ fs[option_case_eq, word_exp_def, IS_SOME_EXISTS]
+         \\  Cases_on `v1` \\ fs[option_case_eq]
+         \\ EVERY_CASE_TAC
+         \\ fs[word_op_def, mem_load_def]
+         \\ rveq
+         \\ fs[set_var_def, get_var_def, mem_store_def]
+         \\ rveq \\ fs[])
+       THEN1 (Cases_on `f`
+         \\ fs[option_case_eq, get_fp_var_def]
+         \\ rveq
+         \\ fs[set_var_def, set_fp_var_def, bool_case_eq]
+         \\ fs[option_case_eq, get_var_def]
+         \\ EVERY_CASE_TAC \\ fs[]
+         \\ rveq \\ fs[]))
+  THEN1
+   (rename [`Get v name`]
+    \\ fs[evaluate_def, opt_code_def, state_rel_def, tree_accurate_def, bool_case_eq, option_case_eq, set_var_def]
+    \\ rveq
+    \\ qexists_tac `0` \\ fs[])
+  THEN1
+   (rename [`Set name v`]
+    \\ fs[evaluate_def, opt_code_def, state_rel_def, tree_accurate_def, bool_case_eq, get_var_def, option_case_eq, set_store_def]
+    \\ rveq \\ qexists_tac `0` \\ fs[])
+  THEN1
+   (rename[`Tick`]
+    \\ fs[evaluate_def, opt_code_def, state_rel_def, tree_accurate_def, bool_case_eq, empty_env_def, dec_clock_def]
+    \\ qexists_tac `0` \\ fs[])
+  THEN1
    (rename [`Seq p1 p2`]
-    \\ once_rewrite_tac [opt_code_def] \\ simp []
-    \\ TOP_CASE_TAC
+    \\ Cases_on `opt_code (Seq p1 p2) tree = Seq (opt_code p1 tree) (opt_code p2 tree)`
     THEN1
      (fs [evaluate_def]
       \\ Cases_on `evaluate (p1,s)` \\ fs []
@@ -89,9 +179,228 @@ Proof
       \\ qpat_x_assum `_ = (NONE,t1)` assume_tac
       \\ drule (GEN_ALL stackPropsTheory.evaluate_add_clock)
       \\ fs [])
-    \\ cheat)
+    \\ pop_assum mp_tac
+    \\ rewrite_tac[opt_code_Seq]
+    \\ TOP_CASE_TAC \\ fs[]
+    \\ TOP_CASE_TAC \\ fs[]
+    \\ TOP_CASE_TAC \\ fs[]
+    THEN1
+      (once_rewrite_tac[opt_code_def] \\ fs[])
+    \\ disch_then kall_tac
+    \\ fs[] \\ rveq
+    \\ fs[evaluate_def]
+    \\ Cases_on `s.use_stack` \\ fs[]
+    \\ Cases_on `LENGTH s.stack < x + s.stack_space` \\ fs[]
+    \\ Cases_on `find_code (INL x') s.regs s.code` \\ fs[]
+    \\ Cases_on `s.clock = 0` \\ fs[]
+    THEN1
+      rveq \\ fs[]
+      \\ fs[new_mem_def]
+      \\ rw[] \\ fs[evaluate_def, state_rel_def, find_code_def]
+      \\ qpat_assum `code_rel _ _ _` mp_tac
+      \\ simp_tac std_ss [Once code_rel_def]
+      \\ disch_then drule
+      \\ strip_tac
+      \\ qexists_tac `0` \\ fs[empty_env_def]
 
-  \\ cheat
+
+
+    \\ TOP_CASE_TAC
+    THEN1
+      (ntac 2 (pop_assum kall_tac)
+      \\ fs [evaluate_def]
+      \\ Cases_on `evaluate (p1,s)` \\ fs []
+      \\ rename [`evaluate (p1,s) = (res0,s0)`]
+      \\ reverse (Cases_on `res0`)
+      THEN1
+       (fs [] \\ rveq \\ fs []
+        \\ first_x_assum (qspecl_then [`t`,`tree`] mp_tac)
+        \\ fs [] \\ strip_tac
+        \\ qexists_tac `ck` \\ fs [])
+      \\ fs []
+      \\ first_x_assum (qspecl_then [`t`,`tree`] mp_tac)
+      \\ fs [] \\ strip_tac
+      \\ first_x_assum (qspecl_then [`t1`,`tree`] mp_tac)
+      \\ fs [] \\ strip_tac
+      \\ qexists_tac `ck+ck'`
+      \\ qpat_x_assum `_ = (NONE,t1)` assume_tac
+      \\ drule (GEN_ALL stackPropsTheory.evaluate_add_clock)
+      \\ fs [])
+
+    TOP_CASE_TAC
+
+
+
+
+
+)
+  THEN1
+   (rename [`Return n m`]
+    \\ fs[evaluate_def, opt_code_def, get_var_def, option_case_eq]
+    \\ EVERY_CASE_TAC \\ fs[]
+    \\ fs[state_rel_def] \\ rveq \\ rfs[])
+  THEN1
+   (rename [`Raise n`]
+    \\ fs[evaluate_def, opt_code_def, option_case_eq, get_var_def]
+    \\ EVERY_CASE_TAC
+      THEN1 (fs[])
+      THEN1 (fs[state_rel_def] \\ rveq \\ fs[]))
+  THEN1
+   (rename [`If cmp r1 ri c1 c2`]
+    \\ once_rewrite_tac [opt_code_def] \\ fs[]
+    \\ fs[evaluate_def, get_var_def, option_case_eq, bool_case_eq]
+    \\ rveq \\ fs[] \\ rfs[]
+    \\ `s.regs = t.regs` by fs[state_rel_def] \\ fs[]
+    \\ `get_var_imm ri t = get_var_imm ri s` by (Cases_on `ri`
+        \\ fs[state_rel_def, get_var_imm_def, get_var_def])
+    \\ fs[]
+    \\ qpat_x_assum `(_,_) = _` (assume_tac o GSYM)
+    \\ first_x_assum drule
+    \\ rpt (disch_then drule)
+    \\ strip_tac \\ qexists_tac `ck` \\ fs[])
+  THEN1
+   (rename [`While cmp r1 ri c1`]
+    \\ once_rewrite_tac [opt_code_def]
+    \\ fs[evaluate_def, option_case_eq, word_loc_case_eq]
+    \\ reverse (Cases_on `word_cmp cmp x y`) \\ fs[]
+      THEN1 (rw[PULL_EXISTS]
+        \\ `s.regs = t.regs` by fs[state_rel_def] \\ fs[]
+        \\ `get_var_imm ri t = get_var_imm ri s` by (Cases_on `ri`
+        \\ fs[state_rel_def, get_var_imm_def, get_var_def])
+        \\ fs[] \\ fs[get_var_def]
+        \\ qexists_tac `0` \\ fs[state_rel_def])
+      THEN1 (rw[PULL_EXISTS]
+        \\ `s.regs = t.regs` by fs[state_rel_def] \\ fs[]
+        \\ `get_var_imm ri t = get_var_imm ri s` by (Cases_on `ri`
+        \\ fs[state_rel_def, get_var_imm_def, get_var_def]))
+        \\ fs[get_var_def]
+        \\ pairarg_tac \\ fs[bool_case_eq]
+        \\ rw[] \\ fs[] \\ rfs[]
+        THEN1
+         (first_x_assum drule
+          \\ disch_then drule
+          \\ rw[]
+          \\ qexists_tac `ck` \\ qexists_tac `t1` \\ fs[])
+        THEN1
+         (first_x_assum drule
+         \\ disch_then drule
+         \\ rw[]
+         \\ qexists_tac `ck` \\ qexists_tac `empty_env t1` \\ fs[state_rel_def]
+         \\ fs[empty_env_def])
+       THEN1
+         (rfs[]
+          \\ qpat_x_assum `(_,_) = _` (assume_tac o GSYM)
+          \\ first_x_assum drule
+          \\ rpt (disch_then drule)
+          \\ rw[]
+          \\ `state_rel (dec_clock s1') (dec_clock t1)` by fs [state_rel_def, dec_clock_def]
+          \\ first_x_assum drule
+          \\ rpt (disch_then drule)
+          \\ rw[]
+          \\ qexists_tac `ck + ck'` \\ fs[]
+          \\ `t1.clock = s1'.clock` by fs [state_rel_def]
+          \\ fs[]
+          \\ qexists_tac `dec_clock t1'` \\ fs[]
+          \\ qpat_x_assum `evaluate (opt_code _ _, _) = (NONE, _)` assume_tac
+    \\ drule (GEN_ALL stackPropsTheory.evaluate_add_clock)
+          \\ disch_then (qspec_then `ck'` mp_tac) \\ simp[]
+          \\ rw[] \\ fs[STOP_def]
+          \\ qpat_x_assum `evaluate (opt_code (While _ _ _ _) _, _) = _` mp_tac
+          \\ once_rewrite_tac [opt_code_def] \\ fs[]
+          \\ cheat)
+          )
+  THEN1
+   (rename [`JumpLower r1 r2 dest`]
+    \\ once_rewrite_tac [opt_code_def] \\ fs[evaluate_def]
+    \\ fs[option_case_eq]
+    \\ Cases_on `v6` \\ fs[option_case_eq]
+    \\ Cases_on `v14` \\ fs[bool_case_eq, option_case_eq]
+    \\ fs[get_var_def, state_rel_def]
+    \\ EVERY_CASE_TAC \\ fs[]
+    \\ cheat)
+  THEN1
+   (rename [`Call ret dest handler`]
+    \\ once_rewrite_tac [opt_code_def] \\ fs[evaluate_def]
+    \\ Cases_on `ret` \\ fs[option_case_eq, bool_case_eq]
+    \\ fs[state_rel_def]
+    \\ cheat)
+  THEN1
+   (rename [`Install ptr len dptr dlen ret`]
+    \\ fs[evaluate_def, opt_code_def]
+    \\ fs[option_case_eq]
+    \\ Cases_on `v14` \\ fs[option_case_eq]
+    \\ Cases_on `v26` \\ fs[option_case_eq]
+    \\ Cases_on `v38` \\ fs[option_case_eq]
+    \\ Cases_on `v46` \\ fs[]
+    \\ fs[get_var_def, state_rel_def]
+    \\ pairarg_tac \\ fs[]
+    \\ pairarg_tac \\ fs[option_case_eq]
+    \\ Cases_on `v12` \\ fs[]
+    \\ Cases_on `v10` \\ fs[]
+    \\ Cases_on `progs'` \\ fs[option_case_eq]
+    \\ Cases_on `v9` \\ fs[]
+    \\ Cases_on `h` \\ fs[bool_case_eq]
+    \\ rveq \\ fs[]
+    \\ cheat)
+  THEN1
+   (rename [`CodeBufferWrite r1 r2`]
+    \\ fs[evaluate_def, opt_code_def, option_case_eq]
+    \\ Cases_on `v5` \\ fs[option_case_eq]
+    \\ Cases_on `v13` \\ fs[option_case_eq]
+    \\ fs[get_var_def, state_rel_def]
+    \\ EVERY_CASE_TAC \\ fs[code_rel_def]
+    \\ cheat)
+  THEN1
+   (rename [`DataBufferWrite r1 r2`]
+    \\ fs[evaluate_def, opt_code_def, bool_case_eq, option_case_eq]
+    \\ Cases_on `v5` \\ fs[option_case_eq]
+    \\ Cases_on `v13` \\ fs[option_case_eq, state_rel_def, get_var_def]
+    \\ cheat)
+  THEN1
+   (rename [`FFI ffi_index ptr len ptr2 len2 ret`]
+    \\ fs[evaluate_def, opt_code_def, option_case_eq]
+    \\ Cases_on `v7` \\ fs[option_case_eq]
+    \\ Cases_on `v19` \\ fs[option_case_eq]
+    \\ Cases_on `v31` \\ fs[option_case_eq]
+    \\ Cases_on `v39` \\ fs[option_case_eq, get_var_def, state_rel_def]
+    \\ EVERY_CASE_TAC \\ fs[]
+    \\ rveq \\ fs[])
+  THEN1
+   (rename [`LocValue r l1 l2`]
+    \\ fs[evaluate_def, opt_code_def, bool_case_eq, state_rel_def, set_var_def]
+    \\ cheat)
+  THEN1
+   (rename [`StackAlloc n`]
+    \\ fs[evaluate_def, opt_code_def, bool_case_eq, state_rel_def, empty_env_def])
+  THEN1
+   (rename [`StackFree n`]
+    \\ fs[evaluate_def, opt_code_def, bool_case_eq, state_rel_def])
+  THEN1
+   (rename [`StackLoad r n`]
+    \\ fs[evaluate_def, opt_code_def, bool_case_eq, state_rel_def, set_var_def])
+  THEN1
+   (rename [`StackLoadAny r rn`]
+    \\ fs[evaluate_def, opt_code_def, bool_case_eq, state_rel_def, get_var_def]
+    \\ EVERY_CASE_TAC \\ fs[set_var_def])
+  THEN1
+   (rename [`StackStore r n`]
+    \\ fs[evaluate_def, opt_code_def, bool_case_eq, state_rel_def, get_var_def]
+    \\ EVERY_CASE_TAC \\ fs[])
+  THEN1
+   (rename [`StackStoreAny r rn`]
+    \\ fs[evaluate_def, opt_code_def, bool_case_eq, state_rel_def, get_var_def]
+    \\ EVERY_CASE_TAC \\ fs[])
+  THEN1
+   (rename [`StackGetSize r`]
+    \\ fs[evaluate_def, opt_code_def, bool_case_eq, state_rel_def, set_var_def])
+  THEN1
+   (rename [`StackSetSize r`]
+    \\ fs[evaluate_def, opt_code_def, bool_case_eq, state_rel_def, get_var_def]
+    \\ EVERY_CASE_TAC \\ fs[set_var_def])
+  THEN1
+   (rename [`BitmapLoad r v`]
+    \\ fs[evaluate_def, opt_code_def, bool_case_eq, state_rel_def, get_var_def]
+    \\ EVERY_CASE_TAC \\ fs[set_var_def])
 QED;
 
 val _ = export_theory();
